\documentclass[10pt,letterpaper]{article}
\usepackage{fullpage}
\usepackage[top=1.75cm, bottom=4cm, left=2.5cm, right=2.5cm]{geometry}
\usepackage{amsmath,amsthm,amsfonts,amssymb,amscd}
\usepackage{lastpage}
\usepackage{enumerate}
\usepackage{fancyhdr}
\usepackage{mathrsfs}
\usepackage{xcolor}
\usepackage{graphicx}
\usepackage{listings}
\usepackage{hyperref}
\usepackage{tcolorbox}
\usepackage{bbm}

\hypersetup{%
colorlinks=true,
linkcolor=blue,
linkbordercolor={0 0 1}
}

\renewcommand\lstlistingname{Algorithm}
\renewcommand\lstlistlistingname{Algorithms}
\def\lstlistingautorefname{Alg.}

\lstdefinestyle{Python}{
  language        = Python,
  frame           = lines,
  basicstyle      = \footnotesize,
  keywordstyle    = \color{blue},
  stringstyle     = \color{green},
  commentstyle    = \color{red}\ttfamily
}

\setlength{\parindent}{0.0in}
\setlength{\parskip}{0.05in}

\newcommand\course{Math 522}
\newcommand\instructor{Dr. Whitehead}
\newcommand\hwnumber{}
\newcommand\name{Jake Callahan, McKay Harward, Taylor Paskett, Isaac Robbins, Mingyan Zhao}
\newtcolorbox{cbox}[3][]
{
  colframe = #2!25,
  colback  = #2!10,
  coltitle = #2!20!black,
  title    = {#3},
  #1,
}

\pagestyle{fancyplain}
\headheight 32pt
\lhead{\name \\ \today}
\chead{\textbf{\Large Final Project \hwnumber}}
\rhead{\course \\ \instructor}
\lfoot{}
\cfoot{}
\rfoot{\small\thepage}
\headsep 1.5em

\begin{document}

TODO

\begin{equation}
\begin{aligned}
p(X=x, \Psi, k | Y=y) \propto & \\
\frac{1}{\sqrt{2 \pi \sigma_{x_{s}}^{2}}} \exp \left\{-\frac{1}{2} \sum_{s \in \Omega}\left(\frac{y_{s}-\mu_{x_{s}}}{\sigma_{x_{s}}}\right)^{2}\right\} \\
\times \frac{\exp \left\{-\sum_{s \in \Omega}\left(\beta_{x_{s}}^{(0)}+\beta^{(1)} V\left(x_{s}, \eta_{s}\right)\right)\right\}}{\prod_{s \in \Omega} \sum_{c \in \Lambda} \exp \left\{-\left(\beta_{c}^{(0)}+\beta^{(1)} V\left(c, \eta_{s}\right)\right)\right\}} \\
\times p_{r}\left(\beta^{(1)}\right) p_{r}(k) \prod_{c \in \Lambda} p_{r}\left(\mu_{c}\right) p_{r}\left(\sigma_{c}\right) p_{r}\left(\beta_{c}^{(0)}\right)
\end{aligned}
\end{equation}


\begin{equation}
\begin{aligned}
p\left(x_{s}=c |\right.&\left.y_{s}, \eta_{c}, \Psi_{c}\right) \propto \\
& \frac{1}{\sqrt{2 \pi \sigma_{c}^{2} T_{t}}} \exp \left\{-\frac{1}{T_{t}}\left[\frac{1}{2}\left(\frac{y_{s}-\mu_{c}}{\sigma_{c}}\right)^{2}+\left(\beta_{c}^{(0)}+\beta^{(1)} V\left(c, \eta_{s}\right)\right)\right]\right\}
\end{aligned}
\end{equation}



\begin{equation}
\begin{aligned}
p\left(\mu_{c}, \sigma_{c} | Y, X\right) & \propto \prod_{s: x_{s}=c} p\left(y_{s} | \mu_{c}, \sigma_{c}\right) p_{r}\left(\mu_{c}\right) p_{r}\left(\sigma_{c}\right) \\
&=\frac{1}{\sigma_{c}\left(2 \pi \sigma_{c}^{2} T_{t}\right)^{n_{c}}} \exp \left\{-\frac{1}{2 T_{t}} \sum_{s: a_{s=c}}\left(\frac{y_{s}-\mu_{c}}{\sigma_{c}}\right)^{2}\right\}
\end{aligned}
\end{equation}


\begin{equation}
\begin{array}{l}
p\left(\beta_{c}^{(0)}, c \in \Lambda | X\right) \\
\quad=p\left(X | \beta_{c}^{(0)}, c \in \Lambda\right) p_{r}\left(\beta_{c}^{(0)}, c \in \Lambda\right) \\
\quad=\prod_{\left(c \in \Lambda, \psi_{\eta}\right)}\left(\frac{\exp \left(-\frac{1}{T_{t}}\left[\beta_{c}^{(0)}+\beta^{(1)} V(c, \eta)\right]\right)}{\sum_{i \in \Lambda} \exp \left(-\frac{1}{T_{t}}\left[\beta_{i}^{(0)}+\beta^{(1)} V(i, \eta)\right]\right)}\right)^{n_{(c, n)}} \\
\quad=\prod_{(c \in \Lambda)}\left(\frac{\exp \left(-\frac{1}{T_{t}}\left[\beta_{c}^{(0)}\right]\right)}{\sum_{i \in \Lambda} \exp \left(-\frac{1}{T_{t}}\left[\beta_{i}^{(0)}\right]\right)}\right)^{n_{c}} \\
\quad \times \prod_{(c \in \Lambda, \psi \eta)}\left(\frac{\exp \left(-\frac{1}{T_{t}}\left[\beta^{(1)} V(c, \eta)\right]\right) \sum_{i \in \Lambda} \exp \left(-\frac{1}{T_{t}}\left[\beta_{i}^{(0)}\right]\right)}{\sum_{i \in \Lambda} \exp \left(-\frac{1}{T_{t}}\left[\beta_{i}^{(0)}+\beta^{(1)} V(i, \eta)\right]\right.}\right)^{n_{(c, n)}}
\end{array}
\end{equation}


\begin{equation}
\begin{aligned}
&\beta_{c 1}^{(0)}=\beta_{c}^{(0)}-T_{t} \ln \left(u_{1}\right) \quad \beta_{c 2}^{(0)}=\beta_{c}^{(0)}-T_{t} \ln \left(1-u_{1}\right)\\
&\begin{array}{l}
\mu_{c 1}=\mu_{c}-u_{2} \sigma_{c} \sqrt{\frac{1-u 1}{u 1}} \quad \mu_{c 2}=\mu_{c}+u_{2} \sigma_{c} \sqrt{\frac{u 1}{1-u 1}} \\
\sigma_{c 1}^{2}=u_{3}\left(1-u_{2}^{2}\right) \sigma_{c}^{2} \frac{1}{u_{1}} \quad \sigma_{c 2}^{2}=\left(1-u_{3}\right)\left(1-u_{2}^{2}\right) \sigma_{c}^{2} \frac{1}{1-u_{1}}
\end{array}
\end{aligned}
\end{equation}


\end{document}
